src/lowparse/LowParseExample5.fst
@@ -1,0 +1,17 @@
+module LowParseExample5
+
+let parse_inner_kind = magic ()
+
+let parse_inner = magic ()
+
+let serialize_inner = magic ()
+
+let serialize_inner_intro = magic ()
+
+let parse_t_kind = magic ()
+
+let parse_t = magic ()
+
+let serialize_t = magic ()
+
+let serialize_t_intro = magic ()
